coq/theories/imperative/ImpSemantics.v
@@ -485,21 +485,14 @@ Definition init_state (inp: llist ascii) (funs: list func): state :=
      output := [];
      steps_done := 0 |}.
 
-Fixpoint lookup_main_imp (fs: list func): option cmd :=
-  match fs with
-  | (Func n ps c) :: fs =>
-    if n =? fun_name_of_string "main" then Some c else lookup_main_imp fs
-  | nil => None
-  end.
-
 Definition eval_from (fuel: nat) (input: llist ascii) (p: prog): (outcome unit * state) :=
   match p with
   | Program funcs =>
     let s0 := init_state input funcs in
-    match lookup_main_imp funcs with
-    | None => crash s0
-    | Some main_c =>
+    match find_fun (fun_name_of_string "main") funcs with
+    | Some ([], main_c) =>
       eval_cmd main_c (EVAL_CMD fuel) s0
+    | _ => crash s0
     end
   end.
 
